\problem{What is the importance of sensitivity analysis in filter design? Explain the sensitivity of the
passive filter.}
The importance of sensitivity analysis in filter design are noted as,
\begin{enumerate}
    \item Sensitivity is used in prediction of behavior of device with change in parameters.
    \item It is used to figure out the extent that errors in elements contribute to entire operation of the network.
    \item It is used to select circuit components and filters for various applications.
    \item Prediction of the difference between a practical filter and nominal design considerations is guided by sensitivity analysis.
    \item Tradeoff for conflicting requirements for low cost and precision are based on sensitivity analysis.
\end{enumerate}
For the sensitivity of passive filter, let us consider a RLC network as,
\begin{figure}[H]
    \centering
    \figRLC
    \caption{Passive RLC network}
    \label{fig:rlc}
\end{figure}

The transfer function of the network shown in Figure~\ref{fig:rlc} is given as,
\begin{equation}
    \begin{aligned}[b]
       & T(s)=\frac{V_2}{V_1}\\
        &\Rightarrow T(s)=\ddfrac{\frac{1}{sC}}{R+sL+\frac{1}{sC}}\\
       & \Rightarrow T(s)=\ddfrac{1}{s^2LC+sRC+1}\\
       & \therefore T(s)=\ddfrac{\frac{1}{LC}}{s^2+s\frac{R}{L}+\frac{1}{LC}}
    \end{aligned}
    \label{eqn:rlc_calc}
\end{equation}
Also, the general equation for a lowpass filter is given as,
\begin{equation}
    T(s)=\ddfrac{H\omega_0^2}{s^2+\frac{\omega_0}{Q}s+\omega_0^2}
    \label{eqn:lp-standard}
\end{equation}
Comparing Equation~\ref{eqn:rlc_calc} and Equation~\ref{eqn:lp-standard}, we get,
\begin{equation*}
    \begin{aligned}
    &\omega_0^2=\frac{1}{LC}\Rightarrow \omega_0=\sqrt{\frac{1}{LC}}=L^{-1/2}C^{-1/2}\\
    &\frac{\omega_0}{Q}=\frac{R}{L}\Rightarrow Q=\frac{1}{R}\sqrt{\frac{L}{C}}=R^{-1}L^{1/2}C^{-1/2}
    \end{aligned}
\end{equation*}
So, we can calculate the following,
\begin{equation}
    \begin{aligned}[b]
        S_L^{\omega_0}&=\left(\frac{L}{\omega_0}\right)\left(\frac{\delta \omega_0}{\delta L}\right)=\left(\frac{L}{\omega_0}\right)\left(\frac{\delta (L^{-1/2}C^{-1/2})}{\delta L}\right)\\
        &=\left(\frac{L}{\omega_0}\right)\left(-\frac{1}{2}L^{-3/2}\right)C^{-1/2}\\
        &=\left(-\frac{1}{2}\right)\frac{L.L^{-3/2}C^{-1/2}}{\omega_0}\\
        &=\left(-\frac{1}{2}\right)\left(\frac{L^{-1/2}L^{-1/2}}{L^{-1/2}C^{-1/2}}\right)=-\frac{1}{2}
    \end{aligned}
\end{equation}

\begin{equation}
    \begin{aligned}[b]
        S_C^{\omega_0}&=\left(\frac{C}{\omega_0}\right)\left(\frac{\delta \omega_0}{\delta C}\right)=\left(\frac{C}{\omega_0}\right)\left(\frac{\delta (L^{-1/2}C^{-1/2})}{\delta C}\right)\\
        &=\left(\frac{C}{\omega_0}\right)\left(-\frac{1}{2}C^{-3/2}\right)L^{-1/2}\\
        &=\left(-\frac{1}{2}\right)\frac{L^{-1/2}C.C^{-3/2}}{\omega_0}\\
        &=\left(-\frac{1}{2}\right)\left(\frac{L^{-1/2}C^{-1/2}}{L^{-1/2}C^{-1/2}}\right)=-\frac{1}{2}
    \end{aligned}
\end{equation}

\begin{equation}
    \begin{aligned}[b]
        S_R^{Q}&=\left(\frac{R}{Q}\right)\left(\frac{\delta Q}{\delta R}\right)=\left(\frac{R}{Q}\right)\left(\frac{\delta (R^{-1}L^{1/2}C^{-1/2})}{\delta Q}\right)\\
        &=\left(\frac{R}{Q}\right)\left(-R^{-2}\right)L^{1/2}C^{-1/2}\\
        &=\left(-1\right)\frac{R.R^{-2}L^{1/2}C^{-1/2}}{Q}\\
        &=\left(-1\right)\left(\frac{R^{-1}L^{1/2}C^{-1/2}}{R^{-1}L^{1/2}C^{-1/2}}\right)=-1
    \end{aligned}
\end{equation}

\begin{equation}
    \begin{aligned}[b]
        S_L^{Q}&=\left(\frac{L}{Q}\right)\left(\frac{\delta Q}{\delta L}\right)=\left(\frac{L}{Q}\right)\left(\frac{\delta (R^{-1}L^{1/2}C^{-1/2})}{\delta Q}\right)\\
        &=\left(\frac{L}{Q}\right)\left(\frac{1}{2}L^{-1/2}\right)R^{-1}C^{-1/2}\\
        &=\left(\frac{1}{2}\right)\frac{L.L^{-1/2}R^{-1}C^{-1/2}}{Q}\\
        &=\left(\frac{1}{2}\right)\left(\frac{R^{-1}L^{1/2}C^{-1/2}}{R^{-1}L^{1/2}C^{-1/2}}\right)=\frac{1}{2}
    \end{aligned}
\end{equation}

\begin{equation}
    \begin{aligned}[b]
        S_C^{Q}&=\left(\frac{C}{Q}\right)\left(\frac{\delta Q}{\delta C}\right)=\left(\frac{C}{Q}\right)\left(\frac{\delta (R^{-1}L^{1/2}C^{-1/2})}{\delta Q}\right)\\
        &=\left(\frac{C}{Q}\right)\left(-\frac{1}{2}C^{-3/2}\right)R^{-1}L^{1/2}\\
        &=\left(-\frac{1}{2}\right)\frac{C.C^{-3/2}R^{-1}L^{1/2}}{Q}\\
        &=\left(-\frac{1}{2}\right)\left(\frac{R^{-1}L^{1/2}C^{-1/2}}{R^{-1}L^{1/2}C^{-1/2}}\right)=-\frac{1}{2}
    \end{aligned}
\end{equation}